omp_compiler/common.v
@@ -3,18 +3,25 @@ From VST.concurrency.openmp_sem Require Export notations HybridMachine.
 From stdpp Require Export base list.
 From compcert Require Export Globalenvs Clight Ctypes Ctypesdefs AST Coqlib Csyntaxdefs.
 Import Csyntaxdefs.CsyntaxNotations.
+From RecordUpdate Require Export RecordSet.
+Export RecordSetNotations.
 Local Open Scope Z_scope.
 Local Open Scope string_scope.
 Local Open Scope csyntax_scope.
 
-Notation "a <|> b" := (match a with Some _ => a | None => b end)
-    (at level 50, left associativity).
+Declare Scope do_notation_scope.
+
+Notation "a <|> b" := (match a with Some _ => a | None => b end) 
+  (at level 50, left associativity) : do_notation_scope.
 
 Section Common.
+  #[local] Open Scope do_notation_scope.
 
   (* assume existence of pthread function names *)
   Definition __opaque_pthread_t : ident := $"_opaque_pthread_t".
   Definition __opaque_pthread_attr_t : ident := $"_opaque_pthread_attr_t".
+  Definition _spawn : ident := $"_spawn".
+  Definition _join_thread : ident := $"_join_thread".
 
   (* FIXME is this used? *)
   Definition adding_ident (identifier: (ident * type)) (existing_list: list (ident * type)):=
@@ -40,5 +47,13 @@ Section Common.
   Definition gen_ident (idents: list ident) : ident * list ident :=
     let i' := ((pos_max idents) + 1)%positive in
     (i', i'::idents).
+
+  #[global] Instance function_settable : Settable function :=
+  settable! mkfunction <fn_return; fn_callconv; fn_params; fn_vars; fn_temps; fn_body>.
+  #[global] Instance composite_definition_settable : Settable composite :=
+    settable! Build_composite <co_su; co_members; co_attr; co_sizeof; co_alignof; co_rank; co_sizeof_pos;co_alignof_two_p; co_sizeof_alignof>.
+(* FIXME *)
+(* #[global] Instance program_settable {F: Type} : Settable (@Ctypes.program F) :=
+  settable! mkprogram <@Ctypes.prog_defs F; prog_public; prog_main;prog_types; prog_comp_env; prog_comp_env_eq>. *)
 
 End Common.
