omp_compiler/par_pass_simu.v
@@ -1,0 +1,5 @@
+From omp_compiler Require Import common par_pass simulation.
+
+Instance par_pass_back_simulation : BackSimulation transl_program.
+Proof.
+Admitted.
